src/proof/yjs_store.v
@@ -1215,7 +1215,7 @@ Proof using Type*.
       rewrite /cell_repr in Hcr_repr.
       iNamed "Htext".
       iDestruct (own_dll_acc _ cells _ _ (Z.to_nat (leftIdx + offset)) ci Hci with "Hdll")
-        as (iv_ci olid_ci orid_ci) "(%Hcloc0 & %Hcl0 & %Hcr0 & %Hcid_ci & %Hccont_ci & %Hcolid_ci & %Hcorid_ci & %Hcflags_ci & %Hccontlen_ci & Hcival & #Hcol & #Hcor & Hback)".
+        as (iv_ci olid_ci orid_ci) "(%Hcloc0 & %Hcl0 & %Hcr0 & %Hcid_ci & %Hccont_ci & %Hcolid_ci & %Hcorid_ci & %Hcflags_ci & %Hccontlen_ci & %Hcpar_ci & Hcival & #Hcol & #Hcor & Hback)".
       iEval (rewrite -Hci_loc) in "Hcival".
       wp_auto.
       iDestruct "Hids_before" as (ibo_s) "[Hibo_ref Hibo_setf]".
@@ -1526,7 +1526,7 @@ Proof using Type*.
       have Hlnn : left_loc ≠ null by rewrite Hll Hcl_loc; exact Hclnn.
       rewrite (bool_decide_eq_false_2 (left_loc = null) Hlnn).
       iDestruct (own_dll_acc _ cells _ _ (Z.to_nat leftIdx) cl Hcl_lookup with "Hdll")
-        as (ivl olidl oridl) "(%Hcloc & %Hcl_l & %Hcr_l & %Hidl & %Hcontl & %Holidl & %Horidl & %Hflagsl & %Hcontlenl & Hcval & #Hcol_l & #Hcor_l & Hback)".
+        as (ivl olidl oridl) "(%Hcloc & %Hcl_l & %Hcr_l & %Hidl & %Hcontl & %Holidl & %Horidl & %Hflagsl & %Hcontlenl & %Hparl & Hcval & #Hcol_l & #Hcor_l & Hback)".
       iEval (rewrite -Hcl_loc) in "Hcval". iEval (rewrite Hll) in "left". wp_auto.
       have Hcr_l' : ivl.(yjs.item.right') = node_loc cells (leftIdx + 1).
       { rewrite Hcr_l. f_equal. rewrite Z2Nat.id; lia. }
@@ -1552,7 +1552,7 @@ Proof using Type*.
         rewrite (bool_decide_eq_false_2 (node_loc cells leftIdx = null) Hlnn'). wp_auto.
         rewrite (bool_decide_eq_false_2 (node_loc cells leftIdx = null) Hlnn').
         iDestruct "Htext" as (yt' tl') "(Hparent & Hdll & %Hlen' & %Hrepr')".
-        iDestruct (own_dll_acc _ cells _ _ (Z.to_nat leftIdx) cl Hcl_lookup with "Hdll") as (ivl2 olidl2 oridl2) "(%Hcloc2 & %Hcl_l2 & %Hcr_l2 & %Hidl2 & %Hcontl2 & %Holidl2 & %Horidl2 & %Hflagsl2 & %Hcontlenl2 & Hcval & #Hcol2 & #Hcor2 & Hback)".
+        iDestruct (own_dll_acc _ cells _ _ (Z.to_nat leftIdx) cl Hcl_lookup with "Hdll") as (ivl2 olidl2 oridl2) "(%Hcloc2 & %Hcl_l2 & %Hcr_l2 & %Hidl2 & %Hcontl2 & %Holidl2 & %Horidl2 & %Hflagsl2 & %Hcontlenl2 & %Hparl2 & Hcval & #Hcol2 & #Hcor2 & Hback)".
         have Hcr_l2' : ivl2.(yjs.item.right') = node_loc cells (leftIdx + 1) by (rewrite Hcr_l2; f_equal; rewrite Z2Nat.id; lia).
         iEval (rewrite -Hcl_loc) in "Hcval". wp_auto. rewrite Hcr_l2'.
         iEval (rewrite Hcl_loc) in "Hcval". iDestruct ("Hback" with "Hcval") as "Hdll".
@@ -1574,7 +1574,7 @@ Proof using Type*.
       iDestruct ("Hbk" with "Hcrval") as "Hdll". iSplitR; [done | iFrame "Hdll"]. }
     have Hrnn : right_loc ≠ null by rewrite Hrl Hcr_loc; exact Hcrnn.
     rewrite (bool_decide_eq_false_2 (right_loc = null) Hrnn).
-    iDestruct (own_dll_acc _ cells _ _ (Z.to_nat rightIdx) cr Hcr_lookup with "Hdll") as (ivr olidr oridr) "(%Hcloc_r & %Hcl_r & %Hcr_r & %Hidr & %Hcontr & %Holidr & %Horidr & %Hflagsr & %Hcontlenr & Hcrval & #Hcol_r & #Hcor_r & Hback)".
+    iDestruct (own_dll_acc _ cells _ _ (Z.to_nat rightIdx) cr Hcr_lookup with "Hdll") as (ivr olidr oridr) "(%Hcloc_r & %Hcl_r & %Hcr_r & %Hidr & %Hcontr & %Holidr & %Horidr & %Hflagsr & %Hcontlenr & %Hparr & Hcrval & #Hcol_r & #Hcor_r & Hback)".
     iEval (rewrite -Hcr_loc) in "Hcrval". iEval (rewrite Hrl) in "right". wp_auto.
     iEval (rewrite Hcr_loc) in "Hcrval". iDestruct ("Hback" with "Hcrval") as "Hdll".
     destruct (decide (leftIdx = -1)) as [Hl0 | HlP].
@@ -1638,7 +1638,7 @@ Proof using Type*.
       have Hlnn : left_loc ≠ null by rewrite Hll Hcl_loc; exact Hclnn.
       rewrite (bool_decide_eq_false_2 (left_loc = null) Hlnn).
       iDestruct (own_dll_acc _ cells _ _ (Z.to_nat leftIdx) cl Hcl_lookup with "Hdll")
-        as (ivl olidl oridl) "(%Hcloc & %Hcl_l & %Hcr_l2 & %Hidl & %Hcontl & %Holidl & %Horidl & %Hflagsl & %Hcontlenl & Hcval & #Hcol_l & #Hcor_l & Hback)".
+        as (ivl olidl oridl) "(%Hcloc & %Hcl_l & %Hcr_l2 & %Hidl & %Hcontl & %Holidl & %Horidl & %Hflagsl & %Hcontlenl & %Hparl & Hcval & #Hcol_l & #Hcor_l & Hback)".
       iEval (rewrite -Hcl_loc) in "Hcval". iEval (rewrite Hll) in "left". wp_auto.
       have Hcr_l' : ivl.(yjs.item.right') = node_loc cells (leftIdx + 1).
       { rewrite Hcr_l2. f_equal. rewrite Z2Nat.id; lia. }
@@ -1664,7 +1664,7 @@ Proof using Type*.
         rewrite (bool_decide_eq_false_2 (node_loc cells leftIdx = null) Hlnn'). wp_auto.
         rewrite (bool_decide_eq_false_2 (node_loc cells leftIdx = null) Hlnn').
         iDestruct "Htext" as (yt' tl') "(Hparent & Hdll & %Hlen' & %Hrepr')".
-        iDestruct (own_dll_acc _ cells _ _ (Z.to_nat leftIdx) cl Hcl_lookup with "Hdll") as (ivl2 olidl2 oridl2) "(%Hcloc2 & %Hcl_l2b & %Hcr_l2b & %Hidl2 & %Hcontl2 & %Holidl2 & %Horidl2 & %Hflagsl2 & %Hcontlenl2 & Hcval & #Hcol2 & #Hcor2 & Hback)".
+        iDestruct (own_dll_acc _ cells _ _ (Z.to_nat leftIdx) cl Hcl_lookup with "Hdll") as (ivl2 olidl2 oridl2) "(%Hcloc2 & %Hcl_l2b & %Hcr_l2b & %Hidl2 & %Hcontl2 & %Holidl2 & %Horidl2 & %Hflagsl2 & %Hcontlenl2 & %Hparl2 & Hcval & #Hcol2 & #Hcor2 & Hback)".
         have Hcr_l2' : ivl2.(yjs.item.right') = node_loc cells (leftIdx + 1) by (rewrite Hcr_l2b; f_equal; rewrite Z2Nat.id; lia).
         iEval (rewrite -Hcl_loc) in "Hcval". wp_auto. rewrite Hcr_l2'.
         iEval (rewrite Hcl_loc) in "Hcval". iDestruct ("Hback" with "Hcval") as "Hdll".
@@ -2043,16 +2043,16 @@ Proof using Type*.
   { eapply YjsArrInvariant_setintegrate; (try eassumption); (try exact _). }
   have Harr'' : insertIdxIfInBounds destIdx itemM arr = take destIdx arr ++ itemM :: drop destIdx arr.
   { rewrite /insertIdxIfInBounds decide_True; [done | rewrite -Hcells_len; exact Hdle]. }
-  have Hcellrepr : cell_repr arr (MkItemCell item_l itemM false) itemM by rewrite /cell_repr //.
-  have Hlen0 : length (cs1m ++ MkItemCell item_l itemM false :: cs2m) = (length cells + 1)%nat.
+  have Hcellrepr : cell_repr arr (MkItemCell item_l itemM false parent) itemM by rewrite /cell_repr //.
+  have Hlen0 : length (cs1m ++ MkItemCell item_l itemM false parent :: cs2m) = (length cells + 1)%nat.
   { rewrite length_app /= (cells_repr_length _ _ _ Hcs1m) (cells_repr_length _ _ _ Hcs2m) length_take length_drop. lia. }
-  have Hnv0 : num_visible (cs1m ++ MkItemCell item_l itemM false :: cs2m) = S (num_visible cells).
+  have Hnv0 : num_visible (cs1m ++ MkItemCell item_l itemM false parent :: cs2m) = S (num_visible cells).
   { rewrite Hcs1eq Hcs2eq. apply num_visible_insert_visible. reflexivity. }
   have Hstart : (ytv <| yjs.yType.len' := w64_word_instance.(word.add) ytv.(yjs.yType.len') (W64 1%nat) |>).(yjs.yType.start') = hd'.
   { simpl. exact Hyts. }
   have Hcs1len : length cs1m = destIdx.
   { rewrite (cells_repr_length _ _ _ Hcs1m) length_take_le; [done | rewrite -Hcells_len; exact Hdle]. }
-  iApply ("HΦ" $! (cs1m ++ MkItemCell item_l itemM false :: cs2m) destIdx (MkItemCell item_l itemM false)).
+  iApply ("HΦ" $! (cs1m ++ MkItemCell item_l itemM false parent :: cs2m) destIdx (MkItemCell item_l itemM false parent)).
   iSplitL "Hparent Hleftdll Hitem Hrightdll2".
   { iExists (ytv <| yjs.yType.len' := w64_word_instance.(word.add) ytv.(yjs.yType.len') (W64 1%nat) |>), tlN.
     iFrame "Hparent".
@@ -2061,15 +2061,15 @@ Proof using Type*.
       have HrightEq : (ivL <| yjs.item.right' := node_loc cells destIdx |>).(yjs.item.right') = node_loc cells destIdx by reflexivity.
       have HleftEq : (ivL <| yjs.item.right' := node_loc cells destIdx |>).(yjs.item.left') = node_loc cells (destIdx - 1).
       { simpl. exact HivLl. }
-      have Hidtr : item_id (ic_item (MkItemCell item_l itemM false)) = toYjsId (ivL <| yjs.item.right' := node_loc cells destIdx |>).(yjs.item.id').
+      have Hidtr : item_id (ic_item (MkItemCell item_l itemM false parent)) = toYjsId (ivL <| yjs.item.right' := node_loc cells destIdx |>).(yjs.item.id').
       { rewrite /= HitemM /= HivLid Hiv2id Hid //. }
-      have Hconttr : content (ic_item (MkItemCell item_l itemM false)) = toContent (ivL <| yjs.item.right' := node_loc cells destIdx |>).(yjs.item.content').
+      have Hconttr : content (ic_item (MkItemCell item_l itemM false parent)) = toContent (ivL <| yjs.item.right' := node_loc cells destIdx |>).(yjs.item.content').
       { rewrite /= HitemM /= HivLc Hiv2con Hcontent //. }
-      have Holtr : origin_id (origin (ic_item (MkItemCell item_l itemM false))) = toYjsId <$> oleft.
+      have Holtr : origin_id (origin (ic_item (MkItemCell item_l itemM false parent))) = toYjsId <$> oleft.
       { rewrite /= HitemM /= Hlpo -Hin_l2 //. }
-      have Hortr : origin_id (rightOrigin (ic_item (MkItemCell item_l itemM false))) = toYjsId <$> oright.
+      have Hortr : origin_id (rightOrigin (ic_item (MkItemCell item_l itemM false parent))) = toYjsId <$> oright.
       { rewrite /= HitemM /= Hrpo -Hin_r2 //. }
-      iApply (own_dll_insert_middle (DfracOwn 1) cs1m cs2m (MkItemCell item_l itemM false)
+      iApply (own_dll_insert_middle (DfracOwn 1) cs1m cs2m (MkItemCell item_l itemM false parent)
                 (ivL <| yjs.item.right' := node_loc cells destIdx |>) oleft oright
                 hd' tlN (node_loc cells (destIdx - 1)) (node_loc cells destIdx)
                 Hitem_nn HleftEq HrightEq Hidtr Hconttr Holtr Hortr Hflv Hclv).
@@ -2090,7 +2090,7 @@ Proof using Type*.
   (* the splice grows the cell list by exactly the new cell: [cs1m = take destIdx
      cells], [cs2m = drop destIdx cells], so [cs1m ++ c :: cs2m ≡ₚ cells ++ [c]]. *)
   iPureIntro. rewrite Hcs1eq Hcs2eq.
-  rewrite (Permutation_cons_append (drop destIdx cells) (MkItemCell item_l itemM false)).
+  rewrite (Permutation_cons_append (drop destIdx cells) (MkItemCell item_l itemM false parent)).
   rewrite app_assoc take_drop //.
 Qed.
 
